Clean up map library

src/goose_lang/map_triples.v
@@ -16,6 +16,64 @@ Implicit Types t : ty.
 Implicit Types stk : stuckness.
 Implicit Types off : nat.
 
+(* The model of a map is [gmap u64 val * val] (the second value is the default).
+
+The abstraction relation (actually abstraction function) between a val mv and a
+model m is m = map_val mv.
+
+The models are canonical due to extensionality of gmaps, but the concrete
+representation tracks all insertions (including duplicates). *)
+
+Fixpoint map_val (v: val) : option (gmap u64 val * val) :=
+  match v with
+  | MapConsV k v m =>
+    match map_val m with
+    | Some (m, def) => Some (<[ k := v ]> m, def)
+    | None => None
+    end
+  | MapNilV def => Some (∅, def)
+  | _ => None
+  end.
+
+Definition val_of_map (m_def: gmap u64 val * val) : val :=
+  let (m, def) := m_def in
+  fold_right (λ '(k, v) mv, MapConsV k v mv)
+             (MapNilV def)
+             (map_to_list m).
+
+Theorem map_val_id : forall v m_def,
+    map_val v = Some m_def ->
+    val_of_map m_def = v.
+Proof.
+  induction v; intros [m def]; try solve [ inversion 1 ]; simpl; intros H.
+  - inversion H; subst; clear H.
+    rewrite map_to_list_empty; simpl; auto.
+  - destruct v; try congruence.
+    destruct v1; try congruence.
+    destruct v1_1; try congruence.
+    destruct l; try congruence.
+    destruct_with_eqn (map_val v2); try congruence.
+    specialize (IHv p).
+    destruct p as [m' def'].
+    inversion H; subst; clear H.
+    (* oops, the normal val induction principle is too weak to prove this *)
+Abort.
+
+Definition map_get (m_def: gmap u64 val * val) (k: u64) : (val*bool) :=
+  let (m, def) := m_def in
+  let r := default def (m !! k) in
+  let ok := bool_decide (is_Some (m !! k)) in
+  (r, ok).
+
+Definition map_insert (m_def: gmap u64 val * val) (k: u64) (v: val) : gmap u64 val * val :=
+  let (m, def) := m_def in
+  (<[ k := v ]> m, def).
+
+Definition map_del (m_def: gmap u64 val * val) (k: u64) : gmap u64 val * val :=
+  let (m, def) := m_def in
+  (delete k m, def).
+
+
 Lemma map_get_empty def k : map_get (∅, def) k = (def, false).
 Proof.
   reflexivity.
